indexed_vlsm_projections.v
@@ -2,7 +2,7 @@ From Casper
 Require Import vlsm indexed_vlsm.
 
 
-Definition indexed_vlsm_projection_initial_state_prop
+Definition vlsm_projection_initial_state_prop
   {message : Type}
   `{CV : composed_vlsm_class message}
   (i : index)
@@ -11,24 +11,22 @@ Definition indexed_vlsm_projection_initial_state_prop
   :=
   exists s : initial_state, istate_proj i (proj1_sig s) = proj1_sig is.
 
-Definition indexed_vlsm_projection_initial_state
+Definition vlsm_projection_initial_state
   {message : Type}
   `{CV : composed_vlsm_class message}
   (i : index)
   :=
-  { s : istate i | indexed_vlsm_projection_initial_state_prop i s }.
+  { s : istate i | vlsm_projection_initial_state_prop i s }.
 
-Lemma indexed_vlsm_projection_protocol_state_inhabited
+Lemma vlsm_projection_protocol_state_inhabited
   {message : Type}
   `{CV : composed_vlsm_class message}
   (i : index)
-  : inhabited (indexed_vlsm_projection_initial_state i).
+  : inhabited (vlsm_projection_initial_state i).
 Proof.
   destruct protocol_state_inhabited as [s].
-  remember (istate_proj i (proj1_sig s)) as is.
-  assert (His : exists s, istate_proj i s = is) by (exists (proj1_sig s); subst; reflexivity).
-  remember (exist (fun is : iproto_state i => exists s : state, istate_proj i s = is) is His) as iis.
-  assert (Hiis : indexed_vlsm_projection_initial_state_prop i iis)
+  remember (proj_istate (proj1_sig s) i) as iis.
+  assert (Hiis : vlsm_projection_initial_state_prop i iis)
     by (exists s; subst; reflexivity).
   constructor. exact (exist _ iis Hiis).
 Qed.
@@ -45,7 +43,7 @@ Definition lift_proto_message
   let Hcm := iproto_message_consistent m0 (proj2_sig m) in
   (exist _ m0 Hcm).
 
-Definition indexed_vlsm_projection_initial_message_prop
+Definition vlsm_projection_initial_message_prop
   {message : Type}
   `{CV : composed_vlsm_class message}
   {iproto_message_prop : message -> Prop}
@@ -72,7 +70,7 @@ Definition noneOrAll
   | (Some p) => p
   end.
 
-Definition indexed_vlsm_projection_valid
+Definition vlsm_projection_valid
   {message : Type}
   `{CV : composed_vlsm_class message}
   {iproto_message_prop : message -> Prop}
@@ -94,20 +92,20 @@ Definition indexed_vlsm_projection_valid
     ).
 
 
-Lemma indexed_vlsm_projection_valid_decidable
+Lemma vlsm_projection_valid_decidable
   {message : Type}
   `{CV : composed_vlsm_class message}
   {iproto_message_prop : message -> Prop}
   (iproto_message_consistent : forall m : message, iproto_message_prop m -> proto_message_prop m)
   (i : index)
   : forall (il : ilabel_type i) (isom : istate i * option {m : message | iproto_message_prop m}),
-  {indexed_vlsm_projection_valid iproto_message_consistent i il isom} + {~indexed_vlsm_projection_valid iproto_message_consistent i il isom}.
+  {vlsm_projection_valid iproto_message_consistent i il isom} + {~vlsm_projection_valid iproto_message_consistent i il isom}.
 Admitted.
 
 Require Import ClassicalChoice ClassicalEpsilon.
 
 
-Definition indexed_vlsm_projection_transition
+Definition vlsm_projection_transition
   {message : Type}
   `{CV : composed_vlsm_class message}
   {iproto_message_prop : message -> Prop}
@@ -117,8 +115,8 @@ Definition indexed_vlsm_projection_transition
   (isom : istate i * option {m : message | iproto_message_prop m})
   : istate i * option {m : message | iproto_message_prop m}.
 remember (option_map (lift_proto_message iproto_message_consistent) (snd isom)) as om.
-destruct (indexed_vlsm_projection_valid_decidable iproto_message_consistent i il isom) as [Hv | Hnv].
-- unfold indexed_vlsm_projection_valid in Hv.
+destruct (vlsm_projection_valid_decidable iproto_message_consistent i il isom) as [Hv | Hnv].
+- unfold vlsm_projection_valid in Hv.
   remember (proj1_sig il) as l.
   destruct isom as [is oim].
   apply constructive_indefinite_description in Hv.
@@ -126,15 +124,14 @@ destruct (indexed_vlsm_projection_valid_decidable iproto_message_consistent i il
   simpl in Heqom. rewrite <- Heqom in *.
   remember (transition l (s,om)) as som'.
   destruct som' as [s' om']. simpl in Hmsg.
-  remember (istate_proj i s') as is'. 
-  assert (His' : exists s'', istate_proj i s'' = is') by (exists s'; subst; reflexivity).
+  remember (proj_istate s' i) as is'. 
   destruct om' as [m'|]; simpl in Hmsg.
-  * exact (exist _ is' His', Some (exist _ (proj1_sig m') Hmsg)).
-  * exact (exist _ is' His', None).
+  * exact (is', Some (exist _ (proj1_sig m') Hmsg)).
+  * exact (is', None).
 - exact (fst isom, None).
 Defined.
 
-Definition indexed_vlsm_projection
+Definition vlsm_projection
   {message : Type}
   `{CV : composed_vlsm_class message}
   {iproto_message_prop : message -> Prop}
@@ -149,44 +146,198 @@ Definition indexed_vlsm_projection
   ;   label := ilabel_type i
   ;   proto_message_prop := iproto_message_prop
   ;   proto_message_decidable := iproto_message_decidable
-  ;   initial_state_prop := indexed_vlsm_projection_initial_state_prop i
-  ;   initial_message_prop := indexed_vlsm_projection_initial_message_prop iproto_message_consistent i
-  ;   transition := indexed_vlsm_projection_transition iproto_message_consistent i
-  ;   protocol_state_inhabited := indexed_vlsm_projection_protocol_state_inhabited i
+  ;   initial_state_prop := vlsm_projection_initial_state_prop i
+  ;   initial_message_prop := vlsm_projection_initial_message_prop iproto_message_consistent i
+  ;   transition := vlsm_projection_transition iproto_message_consistent i
+  ;   protocol_state_inhabited := vlsm_projection_protocol_state_inhabited i
   ;   message_inhabited := iproto_message_inhabited
   ;   label_inhabited := ilabel_inhabited
-  ;   valid := indexed_vlsm_projection_valid iproto_message_consistent i
-  ;   valid_decidable := indexed_vlsm_projection_valid_decidable iproto_message_consistent i
+  ;   valid := vlsm_projection_valid iproto_message_consistent i
+  ;   valid_decidable := vlsm_projection_valid_decidable iproto_message_consistent i
   |}.
 
-(* 
+Definition indexed_vlsm_projection_proto_message_prop
+  {index : Set} {message : Type}
+  (IS : index -> VLSM message)
+  (i : index)
+  : message -> Prop
+  :=
+  @proto_message_prop message (IS i).
+
+Definition indexed_vlsm_projection_proto_message
+  {index : Set} {message : Type}
+  (IS : index -> VLSM message)
+  (i : index)
+  : Type
+  :=
+  {m : message | indexed_vlsm_projection_proto_message_prop IS i m}.
+
+Definition indexed_vlsm_projection_proto_message_decidable
+  {index : Set} {message : Type}
+  (IS : index -> VLSM message)
+  (i : index)
+  : forall m : message, {indexed_vlsm_projection_proto_message_prop IS i m} + {~indexed_vlsm_projection_proto_message_prop IS i m}
+  :=
+  @proto_message_decidable message (IS i).
+
+Definition indexed_vlsm_projection_message_inhabited
+  {index : Set} {message : Type}
+  (IS : index -> VLSM message)
+  (i : index)
+  : inhabited (indexed_vlsm_projection_proto_message IS i)
+  :=
+  @message_inhabited message (IS i).
+
+Lemma indexed_vlsm_projection_proto_message_consistent
+  {index : Set} {message : Type} `{Heqd : EqDec index}
+  (IS : index -> VLSM message)
+  (i : index)
+  : forall m : message, indexed_vlsm_projection_proto_message_prop IS i m -> @proto_message_prop message (composed_vlsm IS (inhabits i)) m.
+Proof.
+  unfold indexed_vlsm_projection_proto_message_prop.
+  intros m Hmi.
+  unfold proto_message_prop; simpl. unfold icomposed_proto_message_prop. exists i. assumption.
+Qed.
+
+Lemma indexed_vlsm_projection_label_inhabited
+  {oindex : Set} {message : Type} `{Heqd : EqDec oindex}
+  (IS : oindex -> VLSM message)
+  (i : oindex)
+  : inhabited (@ilabel_type message (composed_vlsm IS (inhabits i)) (@composed_vlsm_class_instance oindex message Heqd IS (inhabits i)) i).
+Proof.
+  destruct (@label_inhabited message (IS i)) as [l].
+  unfold ilabel_type. unfold label; simpl. unfold composed_vlsm_ilabel. unfold icomposed_label.
+  constructor.
+  exists (existT _ i l).
+  reflexivity.
+Qed.
+
+Definition indexed_vlsm_projection
+  {message : Type}
+  {oindex : Set} {message : Type} `{Heqd : EqDec oindex}
+  (IS : oindex -> VLSM message)
+  (i : oindex)
+  : VLSM (message : Type)
+  :=
+  @vlsm_projection message (composed_vlsm IS (inhabits i)) (@composed_vlsm_class_instance oindex message Heqd IS (inhabits i))
+    (indexed_vlsm_projection_proto_message_prop IS i)
+    (indexed_vlsm_projection_proto_message_decidable IS i)
+    (indexed_vlsm_projection_message_inhabited IS i)
+    (indexed_vlsm_projection_proto_message_consistent IS i)
+    i
+    (indexed_vlsm_projection_label_inhabited IS i)
+  .
+
+Lemma indexed_vlsm_constrained_projection_proto_message_consistent
+  {index : Set} {message : Type} `{Heqd : EqDec index}
+  (IS : index -> VLSM message)
+  (constraint : icomposed_label IS -> icomposed_state IS * option (icomposed_proto_message IS) -> Prop)
+  (constraint_decidable : forall (l : icomposed_label IS) (som : icomposed_state IS * option (icomposed_proto_message IS)), {constraint l som} + {~constraint l som})
+  (i : index)
+  : forall m : message, indexed_vlsm_projection_proto_message_prop IS i m -> @proto_message_prop message (composed_vlsm_constrained IS (inhabits i) constraint constraint_decidable) m.
+Proof.
+  unfold indexed_vlsm_projection_proto_message_prop.
+  intros m Hmi.
+  unfold proto_message_prop; simpl. unfold icomposed_proto_message_prop. exists i. assumption.
+Qed.
+
+Lemma indexed_vlsm_constrained_projection_label_inhabited
+  {oindex : Set} {message : Type} `{Heqd : EqDec oindex}
+  (IS : oindex -> VLSM message)
+  (constraint : icomposed_label IS -> icomposed_state IS * option (icomposed_proto_message IS) -> Prop)
+  (constraint_decidable : forall (l : icomposed_label IS) (som : icomposed_state IS * option (icomposed_proto_message IS)), {constraint l som} + {~constraint l som})
+  (i : oindex)
+  : inhabited (@ilabel_type message (composed_vlsm_constrained IS (inhabits i) constraint constraint_decidable) (@composed_vlsm_constrained_instance oindex message Heqd IS (inhabits i) constraint constraint_decidable) i).
+Proof.
+  destruct (@label_inhabited message (IS i)) as [l].
+  unfold ilabel_type. unfold label; simpl. unfold composed_vlsm_ilabel. unfold icomposed_label.
+  constructor.
+  exists (existT _ i l).
+  reflexivity.
+Qed.
+
+Definition indexed_vlsm_constrained_projection
+  {oindex : Set} {message : Type} `{Heqd : EqDec oindex}
+  (IS : oindex -> VLSM message)
+  (constraint : icomposed_label IS -> icomposed_state IS * option (icomposed_proto_message IS) -> Prop)
+  (constraint_decidable : forall (l : icomposed_label IS) (som : icomposed_state IS * option (icomposed_proto_message IS)), {constraint l som} + {~constraint l som})
+  (i : oindex)
+  : VLSM (message : Type)
+  :=
+  @vlsm_projection message
+    (composed_vlsm_constrained IS (inhabits i) constraint constraint_decidable)
+    (@composed_vlsm_constrained_instance oindex message Heqd IS (inhabits i) constraint constraint_decidable)
+    (indexed_vlsm_projection_proto_message_prop IS i)
+    (indexed_vlsm_projection_proto_message_decidable IS i)
+    (indexed_vlsm_projection_message_inhabited IS i)
+    (indexed_vlsm_constrained_projection_proto_message_consistent IS constraint constraint_decidable i)
+    i
+    (indexed_vlsm_constrained_projection_label_inhabited IS constraint constraint_decidable i)
+  .
+
 Lemma protocol_state_projection
   {index : Set} {message : Type} `{Heqd : EqDec index}
   (IS : index -> VLSM message)
   (constraint : icomposed_label IS -> icomposed_state IS * option (icomposed_proto_message IS) -> Prop)
   (constraint_decidable : forall (l : icomposed_label IS) (som : icomposed_state IS * option (icomposed_proto_message IS)), {constraint l som} + {~constraint l som})
   : forall (j : index) (s :  @protocol_state _ (composed_vlsm_constrained IS (inhabits j) constraint constraint_decidable)),
-  @protocol_state_prop _ (indexed_vlsm_projection IS constraint j) (proj1_sig s j).
+  @protocol_state_prop message
+    (indexed_vlsm_constrained_projection IS constraint constraint_decidable j)
+    (@proj_istate
+      message
+      (composed_vlsm_constrained IS (inhabits j) constraint constraint_decidable)
+      (@composed_vlsm_constrained_instance index message Heqd IS (inhabits j) constraint constraint_decidable)
+      (proj1_sig s)
+      j
+    ).
 Proof.
   intro.
-  apply (protocol_state_ind (fun s : @state _ (composed_vlsm_constrained IS (inhabits j) constraint)  => @protocol_state_prop _ (indexed_vlsm_projection IS constraint j) (s j))); intros.
-  - apply protocol_state_prop_iff. left. destruct is as [s His]. simpl.
-    specialize (His j). remember (exist _ (s j) His) as isj.
-    exists isj. subst. reflexivity.
-  - assert (Hps' : @protocol_state_prop message (composed_vlsm_constrained IS (inhabits j) constraint) (fst (protocol_transition l (s, om)))).
-    { apply protocol_state_iff.
-     
+  apply (protocol_state_ind (fun s : @state _ (composed_vlsm_constrained IS (inhabits j) constraint constraint_decidable)  => @protocol_state_prop message
+    (indexed_vlsm_constrained_projection IS constraint constraint_decidable j)
+    (@proj_istate
+      message
+      (composed_vlsm_constrained IS (inhabits j) constraint constraint_decidable)
+      (@composed_vlsm_constrained_instance index message Heqd IS (inhabits j) constraint constraint_decidable)
+      s
+      j
+    ))); intros.
+  - apply protocol_state_prop_iff. left. 
+    remember (@proj_istate
+      message
+      (composed_vlsm_constrained IS (inhabits j) constraint constraint_decidable)
+      (@composed_vlsm_constrained_instance index message Heqd IS (inhabits j) constraint constraint_decidable)
+      (proj1_sig is)
+      j
+    ) as js.
+    unfold initial_state.
+    unfold initial_state_prop; simpl. unfold vlsm_projection_initial_state_prop.
+    assert (His : exists s0 : initial_state, @istate_proj message
+      (composed_vlsm_constrained IS (inhabits j) constraint constraint_decidable)
+      (@composed_vlsm_constrained_instance index message Heqd IS (inhabits j) constraint constraint_decidable)
+       j (proj1_sig s0) = proj1_sig js)
+      by (exists is; subst; reflexivity).
+    exists (exist _ js His); reflexivity.
+  - assert (Hps' : @protocol_state_prop message (composed_vlsm_constrained IS (inhabits j) constraint constraint_decidable) (fst (protocol_transition l (s, om)))).
+    { apply protocol_state_prop_iff. right. exists s. exists l. exists om. split; try assumption. reflexivity. }
     destruct (protocol_transition l (s, om)) as (s', om') eqn:Ht. simpl.
     destruct l as [i li]; destruct s as [s Hps]. destruct om as [[[m Hm] Hpm]|]; simpl in Ht.
     + simpl in Hv. destruct Hv as [Hv Hc]. simpl in Hv.
       destruct (proto_message_decidable m) as [Hpmi | Hpmi]; simpl ; try (inversion Ht; subst; assumption).
+      remember (@proj_istate
+        message
+        (composed_vlsm_constrained IS (inhabits j) constraint constraint_decidable)
+        (@composed_vlsm_constrained_instance index message Heqd IS (inhabits j) constraint constraint_decidable)
+        s
+        i
+      ) as si.
       remember (exist proto_message_prop m Hpmi) as mi.
-      destruct (transition li (s i, Some mi)) as [si' omi'] eqn:Hti.
+(* 
+      destruct (@transition message (indexed_vlsm_constrained_projection IS constraint constraint_decidable j) (existT _ i li)  (si, Some mi)) as [si' omi'] eqn:Hti.
       inversion Ht as [[Htf Htm]].
       destruct (eq_dec j i); try assumption.
       rewrite e; unfold eq_rect_r; unfold eq_rect; unfold eq_sym.
       simpl in Hind. rewrite e in Hind.
-      apply (@next_protocol_state_with_message _ (indexed_vlsm_projection IS constraint i) (s i) si' li mi omi'); try assumption.
+      apply (@next_protocol_state_with_message _ (indexed_vlsm_constrained_projection IS constraint constraint_decidable j) (s i) si' li mi omi'); try assumption.
       * assert (Himi : @initial_message_prop _ (indexed_vlsm_projection IS constraint i) mi).
         { unfold initial_message_prop; simpl. unfold indexed_vlsm_projection_initial_message_prop. subst. simpl.
           simpl in Hpm.
@@ -200,6 +351,6 @@ Proof.
       * split; try assumption.
         
       apply 
-Admitted.  
-
  *)
+
+Admitted.  
